src/Compilers/CommonSubexpressionEliminationInterp.v
@@ -39,8 +39,9 @@ Section symbolic.
           (interp_op : forall s d (opc : op s d), interp_flat_type interp_base_type s -> interp_flat_type interp_base_type d)
           (symbolize_op : forall s d, op s d -> op_code)
           (denote_op : forall s d, op_code -> option (op s d)).
-
   Local Notation symbolic_expr := (symbolic_expr base_type_code op_code).
+  Context (normalize_symbolic_op_arguments : op_code -> symbolic_expr -> symbolic_expr).
+
   Local Notation symbolic_expr_beq := (@symbolic_expr_beq base_type_code op_code base_type_code_beq op_code_beq).
   Local Notation symbolic_expr_lb := (@internal_symbolic_expr_dec_lb base_type_code op_code base_type_code_beq op_code_beq base_type_code_lb op_code_lb).
   Local Notation symbolic_expr_bl := (@internal_symbolic_expr_dec_bl base_type_code op_code base_type_code_beq op_code_beq base_type_code_bl op_code_bl).
@@ -56,9 +57,9 @@ Section symbolic.
 
   Local Notation symbolicify_smart_var := (@symbolicify_smart_var base_type_code op_code).
   Local Notation symbolize_exprf := (@symbolize_exprf base_type_code op_code op symbolize_op).
-  Local Notation csef := (@csef base_type_code op_code base_type_code_beq op_code_beq base_type_code_bl op symbolize_op).
-  Local Notation cse := (@cse base_type_code op_code base_type_code_beq op_code_beq base_type_code_bl op symbolize_op).
-  Local Notation CSE := (@CSE base_type_code op_code base_type_code_beq op_code_beq base_type_code_bl op symbolize_op).
+  Local Notation csef := (@csef base_type_code op_code base_type_code_beq op_code_beq base_type_code_bl op symbolize_op normalize_symbolic_op_arguments).
+  Local Notation cse := (@cse base_type_code op_code base_type_code_beq op_code_beq base_type_code_bl op symbolize_op normalize_symbolic_op_arguments).
+  Local Notation CSE := (@CSE base_type_code op_code base_type_code_beq op_code_beq base_type_code_bl op symbolize_op normalize_symbolic_op_arguments).
   Local Notation SymbolicExprContext := (@SymbolicExprContext base_type_code op_code base_type_code_beq op_code_beq base_type_code_bl).
   Local Notation SymbolicExprContextOk := (@SymbolicExprContextOk base_type_code op_code base_type_code_beq op_code_beq base_type_code_bl base_type_code_lb op_code_bl op_code_lb).
   Local Notation prepend_prefix := (@prepend_prefix base_type_code op).
